update

horn_ice/horn-ice-examples/ex1.dfy
@@ -1,48 +1,68 @@
-class C {
-  function {:existential true} R1(x : int, r: int, x': int, r': int) : bool {
-    //x <= -1 || (-1 < x && x <= 0 && x - x' <= 0 && x' <= 0 && -1 < r - r' && r - r' <= 0) || (-1 < x && 0 < x)  // generated rely
-    x <= -1 || (x == 0 && x'==x && r'==r) || 0 < x  // manual simplification of generated rely
-    //x == 0 ==> x' == 0 && r' == r  // ideal rely
-  }
+function {:existential true} R1(x : int, x': int) : bool {
+  (x <= 1 && x <= -1) || (x <= 1 && -1 < x && x <= 0 && -1 < x' && x' <= 0) || (x <= 1 && -1 < x && 0 < x) || 1 < x
+}
 
+function {:existential true} R2(x : int, x': int) : bool {
+  (-1 < x - x' && x + x' <= -2) || (-1 < x - x' && -2 < x + x' && x - x' <= 0)
+}
+
+class C {
   var x: int
-  var r: int
 
   method T1()
     requires x == 0
     modifies this
-    ensures r == 0
   {
+    var r: int;
     Rely1();
     r := x;
     Rely1();
+    assert r == 0;
   }
 
   method T2()
     modifies this
   {
-    var old_x:int;
+    Rely2();
+    var old_x: int;
     if (x != 0) {
+      Rely2();
       old_x := x;
       x := 1;
-      assert R1(old_x,r,x,r);
+      assert R1(old_x,x);
+      Rely2();
     }
   }
 
   method Rely1()
     modifies this
-    ensures R1(old(x),old(r),x,r)
+    ensures R1(old(x),x)
 
   method ReflexiveR1()
-    ensures R1(old(x),old(r),x,r)
+    ensures R1(old(x),x)
   {}
 
   method TransitiveR1()
-    modifies this 
-    ensures R1(old(x),old(r),x,r)
+    modifies this
+    ensures R1(old(x),x)
   {
     Rely1();
     Rely1();
   }
-  
+
+  method Rely2()
+    modifies this
+    ensures R2(old(x),x)
+
+  method ReflexiveR2()
+    ensures R2(old(x),x)
+  {}
+
+  method TransitiveR2()
+    modifies this
+    ensures R2(old(x),x)
+  {
+    Rely2();
+    Rely2();
+  }
 }
